vera/VerilogToSMT/VerilogToSMTCorrect.v
@@ -140,35 +140,38 @@ Qed.
 Lemma module_item_to_smt_satisfiable
   tag m (mi : Verilog.module_item) inputs outputs :
   disjoint inputs outputs ->
-  forall t regs regs' ρ,
+  forall t regs ρ,
     transfer_module_item tag m inputs outputs mi = inr t ->
-    exec_module_item regs mi = Some regs' ->
     verilog_smt_match_states_partial
       (fun var => List.In var (Verilog.module_item_reads mi ++ Verilog.module_item_writes mi))
-      tag m regs' ρ ->
+      tag m
+      (exec_module_item regs mi) ρ ->
     SMTQueries.term_satisfied_by ρ t.
 Proof.
-  funelim (transfer_module_item tag m inputs outputs mi); intros; monad_inv; [idtac].
+  funelim (transfer_module_item tag m inputs outputs mi); expect 1.
+  intros * Hdisjoint * Hexec Hmatch.
+  monad_inv; expect 1.
   simp exec_module_item exec_statement in *.
   monad_inv.
   unfold SMTQueries.satisfied_by, SMTQueries.term_satisfied_by. repeat constructor.
   simpl.
 
-  edestruct eval_expr_no_exes as [bv_rhs Hbv_rhs]; eauto; [idtac|idtac]. {
+  destruct (eval_expr_no_exes _ regs rhs) as [bv_rhs Hbv_rhs]; expect 2. {
     simp module_item_reads module_item_writes
       statement_reads statement_writes expr_reads
       in *.
-    setoid_rewrite List.in_app_iff in H2.
-    apply verilog_smt_match_states_partial_split_iff in H2.
-    destruct H2.
+    simpl in Hmatch.
+    setoid_rewrite List.in_app_iff in Hmatch .
+    apply verilog_smt_match_states_partial_split_iff in Hmatch.
+    destruct Hmatch as [Hmatch_reads Hmatch_var].
     eapply defined_value_for_set_reg_intro_out with (var:=var). {
       rewrite List.Forall_forall in *.
-      eapply disjoint_r_intro in H; eauto.
+      eapply disjoint_r_intro in Hdisjoint; eauto.
     }
     eapply verilog_smt_match_states_partial_defined_value_for.
     eassumption.
   }
-  apply XBV.to_from_bv_inverse in Hbv_rhs. subst x.
+  apply XBV.to_from_bv_inverse in Hbv_rhs. rewrite Hbv_rhs in *.
 
   erewrite var_to_smt_value with (var := var) (regs := (RegisterState.set_reg var (XBV.from_bv bv_rhs) regs)); eauto; cycle 1.
   {
@@ -186,9 +189,9 @@ Proof.
       simp module_item_reads module_item_writes statement_writes statement_reads expr_reads.
       eauto with datatypes.
     - rewrite List.Forall_forall in *.
-      eapply disjoint_r_intro in H; eauto.
+      eapply disjoint_r_intro in Hdisjoint; eauto.
   }
-  rewrite E. simpl. rewrite XBV.xbv_bv_inverse.
+  rewrite Hbv_rhs. simpl. rewrite XBV.xbv_bv_inverse.
   autodestruct; [|contradiction].
   repeat f_equal. apply BV.bv_eq_reflect. apply eq_rect_eq.
 Qed.
@@ -220,10 +223,10 @@ Lemma module_item_to_smt_valid tag m (mi : Verilog.module_item) inputs outputs :
       verilog_smt_match_states_partial
         (fun var => List.In var (Verilog.module_item_reads mi))
         tag m r1 ρ ->
-      exists r2, exec_module_item r1 mi = Some r2 /\
-              verilog_smt_match_states_partial
-                (fun var => List.In var (Verilog.module_item_reads mi ++ Verilog.module_item_writes mi))
-                tag m r2 ρ.
+          verilog_smt_match_states_partial
+            (fun var => List.In var (Verilog.module_item_reads mi ++ Verilog.module_item_writes mi))
+              tag m
+              (exec_module_item r1 mi) ρ.
 Proof.
   funelim (transfer_module_item tag m inputs outputs mi);
     intros * Hdisjoint * Htransf Hsat * Hmatch1; monad_inv; [idtac].
@@ -231,32 +234,19 @@ Proof.
   simp exec_module_item exec_statement in *.
   monad_inv.
   rewrite smt_eq_sat_iff in Hsat. destruct Hsat as [v [Ht0 Ht1]].
-  edestruct expr_to_smt_valid as [xbv_expr [Heval_expr Hmatch_expr]]; eauto; [idtac].
-  edestruct eval_expr_no_exes;
-    eauto using verilog_smt_match_states_partial_defined_value_for;
-    [idtac].
-  apply_somewhere XBV.bv_xbv_inverse. subst xbv_expr.
-  rewrite Heval_expr.
+  pose proof expr_to_smt_valid as Hvalue_match. insterU Hvalue_match.
+  inv Hvalue_match. simpl.
   edestruct var_to_smt_valid as [xbv_var [Heval_var Hmatch_var]]; eauto.
-  simpl. eexists. split; [reflexivity|].
-  eapply verilog_smt_match_states_partial_split. solve [apply List.in_app_or].
-  - eapply verilog_smt_match_states_partial_set_reg_elim. {
-      eexists. split. { eassumption. }
-      replace (ρ xbv_var).
-      inv Hmatch_expr.
-      apply_somewhere RawXBV.from_bv_injective.
-      repeat f_equal.
-      now apply BV.of_bits_equal.
-    }
-    eassumption.
+  unpack_verilog_smt_match_states_partial.
+  - apply verilog_smt_match_states_partial_set_reg_out; [|assumption].
+    unfold disjoint in *.
+    rewrite List.Forall_forall in *.
+    firstorder.
   - unfold verilog_smt_match_states_partial.
-    intros * Hin.
-    inv Hin; [|crush].
-    exists xbv_var. split. { eassumption. }
-    econstructor.
-    + eassumption.
-    + eapply RegisterState.set_reg_get_in.
-    + eassumption.
+    intros. inv H; [|crush].
+    eexists. split; [eassumption|].
+    econstructor; [eassumption|idtac|econstructor].
+    apply RegisterState.set_reg_get_in.
 Qed.
 
 Definition inputs_of_execution
@@ -282,64 +272,11 @@ Proof.
   some_inv. eauto.
 Qed.
 
-(* TODO: StrFunMap.gsi *)
-
-Lemma exec_statement_reads_has_values_before r1 r2 stmt :
-  exec_statement r1 stmt = Some r2 ->
-  List.Forall (fun n => exists v, r1 n = v) (Verilog.statement_reads stmt).
-Proof.
-  rewrite List.Forall_forall.
-  intros.
-  funelim (exec_statement r1 stmt);
-    clear Heqcall;
-    simp exec_statement in *;
-    try discriminate.
-  crush.
-Qed.
-
-Lemma exec_statement_preserve stmt : forall r1 r2 var,
-  exec_statement r1 stmt = Some r2 ->
-  (~ List.In var (Verilog.statement_writes stmt)) ->
-  r1 var = r2 var.
-Proof.
-  intros * Hexec Hnotin.
-  funelim (exec_statement r1 stmt);
-    clear Heqcall;
-    simp exec_statement in *;
-    try discriminate.
-  monad_inv.
-  rewrite RegisterState.set_reg_get_out by crush.
-  reflexivity.
-Qed.
-
-Lemma exec_module_item_preserve mi : forall r1 r2 var,
-  exec_module_item r1 mi = Some r2 ->
-  (~ List.In var (Verilog.module_item_writes mi)) ->
-  r1 var = r2 var.
-Proof.
-  intros.
-  funelim (exec_module_item r1 mi); simp exec_module_item in *; try discriminate; [idtac].
-  eapply exec_statement_preserve; eauto.
-Qed.
-
-Lemma exec_module_body_preserve procs : forall r1 r2 var,
-  exec_module_body r1 procs = Some r2 ->
-  (~ List.In var (Verilog.module_body_writes procs)) ->
-  r1 var = r2 var.
-Proof.
-  induction procs; intros * Hrun Hin; simp exec_module_body in *.
-  - inv Hrun. reflexivity.
-  - simp module_body_writes in *. rewrite List.in_app_iff in *.
-    monad_inv.
-    transitivity (r var).
-    + eapply exec_module_item_preserve; eauto.
-    + eapply IHprocs; eauto.
-Qed.
-
 Lemma transfer_module_item_inputs tag m inputs outputs mi t :
   transfer_module_item tag m inputs outputs mi = inr t ->
-  List.Forall (fun var => List.In var inputs) (Verilog.module_item_reads mi).
+  list_subset (Verilog.module_item_reads mi) inputs.
 Proof.
+  unfold list_subset.
   funelim (transfer_module_item tag m inputs outputs mi); intros; try discriminate.
   monad_inv.
   simp module_item_reads statement_reads.
@@ -347,8 +284,9 @@ Qed.
 
 Lemma transfer_module_item_outputs tag m inputs outputs mi t :
   transfer_module_item tag m inputs outputs mi = inr t ->
-  List.Forall (fun var => List.In var outputs) (Verilog.module_item_writes mi).
+  list_subset (Verilog.module_item_writes mi) outputs.
 Proof.
+  unfold list_subset.
   funelim (transfer_module_item tag m inputs outputs mi); intros; try discriminate.
   monad_inv.
   simp module_item_writes statement_writes expr_reads.
@@ -357,61 +295,57 @@ Qed.
 
 Lemma transfer_module_body_outputs tag m inputs outputs mis t :
   transfer_module_body tag m inputs outputs mis = inr t ->
-  List.Forall (fun var => List.In var outputs) (Verilog.module_body_writes mis).
+  list_subset (Verilog.module_body_writes mis) outputs.
 Proof.
   funelim (transfer_module_body tag m inputs outputs mis); intros; try discriminate.
   - inv H. simp module_body_writes. constructor.
   - monad_inv.
     simp module_body_writes in *.
-    eapply List.Forall_app.
-    eauto using transfer_module_item_outputs with datatypes.
+    apply list_subset_app.
+    split; eauto using transfer_module_item_outputs with datatypes.
 Qed.
 
 Lemma transfer_module_body_inputs tag m inputs outputs mis t :
   transfer_module_body tag m inputs outputs mis = inr t ->
-  List.Forall (fun var => List.In var inputs) (Verilog.module_body_reads mis).
+  list_subset (Verilog.module_body_reads mis) inputs.
 Proof.
   funelim (transfer_module_body tag m inputs inputs mis); intros; try discriminate.
   - inv H. simp module_body_reads. constructor.
   - simp transfer_module_body module_body_reads in *.
     monad_inv.
-    eapply List.Forall_app.
-    eauto using transfer_module_item_inputs with datatypes.
+    apply list_subset_app.
+    split; eauto using transfer_module_item_inputs with datatypes.
 Qed.
 
 Lemma transfer_module_body_exec_satisfiable inputs outputs body :
-  forall tag (m : VerilogSMTBijection.t) r1 r2 q ρ,
+  forall tag (m : VerilogSMTBijection.t) r1 q ρ,
     disjoint inputs outputs ->
     transfer_module_body tag m inputs outputs body = inr q ->
-    exec_module_body r1 body = Some r2 ->
     verilog_smt_match_states_partial
       (fun var => List.In var (Verilog.module_body_reads body ++ Verilog.module_body_writes body))
-      tag m r2 ρ ->
+      tag m (exec_module_body r1 body) ρ ->
     List.Forall (SMTQueries.term_satisfied_by ρ) q.
 Proof.
   (* generalize dependent (Verilog.module_outputs v). intro outputs.
    * generalize dependent (Verilog.module_inputs v). intro inputs.
    * generalize dependent (Verilog.modBody v). intro body. *)
-  induction body; intros * Hdisjoint Htransfer Hvalid Hmatch; simp module_body_reads module_body_writes transfer_module_body in *; [some_inv; constructor|].
-  simp exec_module_body in Hvalid.
+  induction body; intros * Hdisjoint Htransfer Hmatch; simp module_body_reads module_body_writes transfer_module_body in *; [some_inv; constructor|].
+  simp exec_module_body in Hmatch. simpl in Hmatch.
   monad_inv.
   constructor.
-  - eapply module_item_to_smt_satisfiable with (inputs := inputs).
+  - eapply module_item_to_smt_satisfiable with (inputs := inputs) (regs:=r1).
     all: try eassumption; expect 1.
-    eapply verilog_smt_match_states_partial_change_regs with (r1 := r2). {
+    eapply verilog_smt_match_states_partial_change_regs with (r1 := (exec_module_body (exec_module_item r1 a) body)). {
       intros.
-      rewrite ! List.in_app_iff in *.
-      pose proof transfer_module_item_inputs as Hinputs. insterU Hinputs.
-      pose proof transfer_module_item_outputs as Houtputs. insterU Houtputs.
-      rewrite List.Forall_forall in *.
-      symmetry. eapply exec_module_body_preserve. eassumption.
-      intro Hinbody.
-      destruct H.
-      - eapply disjoint_l_intro with (l:=inputs); eauto; [idtac].
-        pose proof transfer_module_body_outputs as Hbody_outputs.
-        insterU Hbody_outputs. rewrite List.Forall_forall in Hbody_outputs.
-        auto.
-      - eapply disjoint_l_intro; eauto.
+      symmetry. eapply Facts.exec_module_body_preserve; [clear H|apply H].
+      unfold disjoint in *.
+      rewrite ! List.Forall_forall in *.
+      setoid_rewrite List.in_app_iff.
+      setoid_rewrite transfer_module_item_inputs; try eassumption.
+      intros var' [Hvar_read|Hvar_write].
+      - setoid_rewrite transfer_module_body_outputs; try eassumption.
+        eauto.
+      - eauto.
     }
     eapply verilog_smt_match_states_partial_impl; [|eassumption].
     intros. simpl.
@@ -443,117 +377,97 @@ Lemma transfer_module_body_satisfiable v tag (m : VerilogSMTBijection.t) ρ q :
     list_subset (Verilog.module_body_reads (Verilog.modBody v)) (Verilog.module_inputs v) ->
     Permutation (Verilog.module_body_writes (Verilog.modBody v)) (Verilog.module_outputs v) ->
     disjoint (Verilog.module_inputs v) (Verilog.module_outputs v) ->
+    module_items_sorted (Verilog.module_inputs v) (Verilog.modBody v) ->
     transfer_module_body tag m (Verilog.module_inputs v) (Verilog.module_outputs v) (Verilog.modBody v) = inr q ->
     v ⇓ (SMT.execution_of_valuation tag m ρ) ->
     List.Forall (SMTQueries.term_satisfied_by ρ) q.
 Proof.
-  intros * Hwrites_ndup Hreads_subset Hwrites_permute Hdisjoint Htransfer Hvalid.
-  destruct Hvalid as [e' [? [? [? ?]]]].
+  intros * Hwrites_ndup Hreads_subset Hwrites_permute Hdisjoint Hsorted Htransfer Hvalid.
+  destruct Hvalid as [? [? ?]].
   RegisterState.unpack_match_on.
-  repeat unfold mk_initial_state, run_vmodule in *. monad_inv.
-  (* Renaming monad_inv results to consistent names *)
-  match goal with [ H : sort_module_items _ _ = Some ?l |- _ ] =>
-    rename H into Hsort; rename l into sorted
-  end.
-  rename_match (exec_module_body _ sorted = Some _) into Hexec.
-  apply_somewhere sort_module_items_permutation.
-  erewrite <- exec_module_body_permute in Hexec; cycle 1.
-  - eassumption.
-  - eassumption.
-  - rewrite <- Hsort. assumption.
-  - rewrite Hwrites_permute.
-    rewrite Hreads_subset.
-    try symmetry; eassumption.
-  - rewrite <- Hsort.
-    rewrite Hwrites_permute.
-    rewrite Hreads_subset.
-    try symmetry; eassumption.
-  - eapply transfer_module_body_exec_satisfiable; eauto.
-    apply transfer_module_body_inputs in Htransfer.
-    rewrite List.Forall_forall in Htransfer.
-    apply execution_match_on_verilog_smt_match_states_partial.
-    + RegisterState.unpack_defined_value_for.
-      * setoid_replace
-	  (fun var => List.In var (Verilog.module_body_reads (Verilog.modBody v))) with
-	  (fun var => List.In var (Verilog.module_inputs v))
-	  by (unfold pointwise_relation, Basics.impl; apply Htransfer).
-        setoid_rewrite H2.
-	apply execution_of_valuation_has_value_defined_value.
-	assumption.
-      * setoid_rewrite Hwrites_permute.
-        setoid_rewrite H3.
-        apply execution_of_valuation_has_value_defined_value.
-	assumption. 
-    + RegisterState.unpack_match_on.
-      * eapply RegisterState.match_on_impl. now eapply Htransfer. eassumption.
-      * setoid_rewrite Hwrites_permute. eassumption.
+  rename_match (_ =( Verilog.module_inputs _ )= _) into Hmatch_inputs.
+  rename_match (_ =( Verilog.module_outputs _ )= _) into Hmatch_outputs.
+  repeat unfold mk_initial_state, run_vmodule in *.
+  rewrite ! sort_module_items_stable in * by eassumption.
+  rewrite RegisterState.limit_to_regs_twice in *.
+  eapply transfer_module_body_exec_satisfiable; eauto.
+  (* apply transfer_module_body_inputs in Htransfer.
+   * rewrite List.Forall_forall in Htransfer. *)
+  apply execution_match_on_verilog_smt_match_states_partial.
+  + RegisterState.unpack_defined_value_for.
+    * setoid_rewrite Hreads_subset.
+      rewrite Hmatch_inputs.
+      apply execution_of_valuation_has_value_defined_value.
+      assumption.
+    * setoid_rewrite Hwrites_permute.
+      setoid_rewrite Hmatch_outputs.
+      apply execution_of_valuation_has_value_defined_value.
+      assumption. 
+  + RegisterState.unpack_match_on.
+    * setoid_rewrite Hreads_subset. apply Hmatch_inputs.
+    * setoid_rewrite Hwrites_permute. apply Hmatch_outputs.
+Qed.
+
+Global Instance verilog_smt_match_states_partial_proper C :
+  Proper
+    (eq ==> eq ==> (RegisterState.match_on C) ==> eq ==> iff)
+    (verilog_smt_match_states_partial C).
+Proof.
+  unfold verilog_smt_match_states_partial.
+  repeat intro. subst.
+  split; intros.
+  - edestruct H as [smtName [Hlookup Hmatch]]; [eassumption|].
+    eexists. split; [eauto|].
+    inv Hmatch. econstructor; eauto.
+    now rewrite <- H1.
+  - edestruct H as [smtName [Hlookup Hmatch]]; [eassumption|].
+    eexists. split; [eauto|].
+    inv Hmatch. econstructor; eauto.
+    now rewrite H1.
 Qed.
 
 Lemma transfer_module_body_exec_valid inputs outputs body : forall tag m ρ q,
     disjoint inputs outputs ->
+    list_subset (Verilog.module_body_writes body) outputs ->
     transfer_module_body tag m inputs outputs body = inr q ->
     List.Forall (SMTQueries.term_satisfied_by ρ) q ->
     forall r1,
       verilog_smt_match_states_partial
         (fun var => List.In var inputs)
         tag m r1 ρ ->
-      exists r2,
-        exec_module_body r1 body = Some r2 /\
           verilog_smt_match_states_partial
             (fun var =>
                List.In var (inputs ++ Verilog.module_body_writes body)
-            ) tag m r2 ρ.
+            ) tag m (exec_module_body r1 body) ρ.
 Proof.
-  induction body; intros * Hdisjoint Htransfer Hsat * Hmatch1;
-    simpl in *;
-    simp module_body_reads module_body_writes transfer_module_body exec_module_body in *;
-    autorewrite with list;
-    [crush|].
+  induction body.
+  all: intros * Hdisjoint Houtputs_in Htransfer Hsat * Hmatch1.
+  all: simpl in *.
+  all: simp module_body_reads module_body_writes transfer_module_body exec_module_body in *.
+  all: autorewrite with list.
+  1: crush. all: expect 1.
+  unpack_list_subset.
+  disjoint_saturate.
   monad_inv. inv Hsat.
-  edestruct module_item_to_smt_valid with (inputs := inputs) as [r_mid [Heval_mid Hmatch_mid]]; try eauto; [|]. {
-    eapply verilog_smt_match_states_partial_impl; [|eassumption].
-    simpl. intros.
-    unfold list_subset in l.
-    rewrite List.Forall_forall in l.
-    auto.
-  }
-  rewrite Heval_mid. simpl.
-  edestruct IHbody with (r1 := r_mid) as [r2 [Heval2 Hmatch2]]; try eassumption. {
-    eapply verilog_smt_match_states_partial_change_regs. {
-      (* TODO: Different name for the two `exec_module_item_preserve`s *)
-      intros. eapply VerilogToSMTCorrect.exec_module_item_preserve; [eassumption|].
-      intro.
-      pose proof transfer_module_item_outputs as Houtputs. insterU Houtputs.
-      pose proof transfer_module_body_inputs as Hinputs. insterU Hinputs.
-      rewrite List.Forall_forall in *.
-      eapply disjoint_l_intro with (l:=inputs); eauto.
-    }
-    eapply verilog_smt_match_states_partial_impl; [|eassumption]. {
-      simpl. intros.
-      assumption.
-    }
-  }
-  exists r2.
-  split. eassumption.
-  eapply verilog_smt_match_states_partial_split; cycle 1.
-  - eapply verilog_smt_match_states_partial_change_regs; [|eapply Hmatch_mid].
-    intros.
-    rewrite ! List.in_app_iff in *.
-    pose proof transfer_module_item_inputs as Hinputs. insterU Hinputs.
-    pose proof transfer_module_item_outputs as Houtputs. insterU Houtputs.
-    rewrite List.Forall_forall in *.
-    (* TODO: Different name for the two `exec_module_item_preserve`s *)
-    eapply VerilogToSMTCorrect.exec_module_body_preserve. eassumption.
-    intro Hinbody.
-    destruct H.
-    + eapply disjoint_l_intro with (l:=inputs); eauto; [idtac].
-      pose proof transfer_module_body_outputs as Hbody_outputs.
-      insterU Hbody_outputs. rewrite List.Forall_forall in Hbody_outputs.
-      auto.
-    + eapply disjoint_l_intro; eauto.
-  - eapply Hmatch2.
-  - repeat setoid_rewrite List.in_app_iff. intros.
-    intuition assumption.
+  rename_match (list_subset (Verilog.module_item_writes a) outputs) into Hitem_writes.
+  rename_match (list_subset (Verilog.module_item_reads a) inputs) into Hitem_reads.
+  eapply verilog_smt_match_states_partial_split with
+    (C1 := fun var => List.In var (inputs ++ Verilog.module_body_writes body))
+    (C2 := fun var => List.In var (Verilog.module_item_writes a)).
+  - repeat setoid_rewrite List.in_app_iff. intros ? [? | [? | ?]]; auto.
+  - simpl.
+    eapply IHbody; try eassumption; expect 1.
+    setoid_rewrite <- Facts.exec_module_item_preserve; [assumption|].
+    setoid_rewrite Hitem_writes. assumption.
+  - simpl.
+    setoid_rewrite <- Facts.exec_module_body_preserve; [|assumption].
+    eapply verilog_smt_match_states_partial_impl; cycle 1.
+    + eapply module_item_to_smt_valid; cycle 1.
+      * eassumption.
+      * assumption.
+      * setoid_rewrite Hitem_reads. assumption.
+      * assumption.
+    + setoid_rewrite List.in_app_iff. auto.
 Qed.
 
 Lemma defined_value_for_has_value_for C e :
@@ -573,40 +487,52 @@ Lemma transfer_module_body_valid tag m v ρ q :
   valid_execution v (SMT.execution_of_valuation tag m ρ).
 Proof.
   intros * Hsorted Hinputs_subset Houtputs_permute Hnodup_writes Hdisjoint Htransfer Hhas_vars Hsat.
-  edestruct transfer_module_body_exec_valid
-    with (r1 := RegisterState.limit_to_regs (Verilog.module_inputs v) (SMT.execution_of_valuation tag m ρ))
-    as [final [H1 H2]].
-  - eassumption.
-  - eassumption.
-  - eassumption.
-  - eapply verilog_smt_match_states_partial_change_regs
-      with (r1 := SMT.execution_of_valuation tag m ρ). {
-      intros.
-      unfold list_subset in Hinputs_subset.
-      rewrite List.Forall_forall in Hinputs_subset.
-      unfold RegisterState.limit_to_regs.
-      autodestruct; crush.
-    }
+  (* pose proof transfer_module_body_exec_valid
+   *   with (r1 := (SMT.execution_of_valuation tag m ρ) // (Verilog.module_inputs v)). *)
+  (* - eassumption.
+   * - rewrite Houtputs_permute. reflexivity.
+   * - eassumption.
+   * - eassumption.
+   * - eapply verilog_smt_match_states_partial_change_regs
+   *     with (r1 := SMT.execution_of_valuation tag m ρ). {
+   *     intros.
+   *     unfold list_subset in Hinputs_subset.
+   *     rewrite List.Forall_forall in Hinputs_subset.
+   *     unfold RegisterState.limit_to_regs.
+   *     autodestruct; crush.
+   *   }
+   *   apply verilog_smt_match_states_execution_of_valuation_same.
+   *   intros. apply Hhas_vars. apply Verilog.module_input_in_vars. assumption.
+   * - admit. *)
+  unfold valid_execution.
+  (* destruct Hsortable as [sorted Hsort]. *)
+  repeat unfold mk_initial_state, run_vmodule in *.
+  rewrite sort_module_items_stable by assumption. simpl.
+  rewrite RegisterState.limit_to_regs_twice.
+  unpack_goal.
+  - apply defined_value_for_has_value_for.
+    eapply verilog_smt_match_states_partial_execution_defined_value_for.
     apply verilog_smt_match_states_execution_of_valuation_same.
     intros. apply Hhas_vars. apply Verilog.module_input_in_vars. assumption.
-  - unfold valid_execution.
-    (* destruct Hsortable as [sorted Hsort]. *)
-    repeat unfold mk_initial_state, run_vmodule in *.
-    rewrite sort_module_items_stable by assumption. simpl.
-    eexists. unpack_goal.
-    + rewrite RegisterState.limit_to_regs_twice.
-      eassumption.
-    + apply defined_value_for_has_value_for.
-      eapply verilog_smt_match_states_partial_execution_defined_value_for.
+  - apply defined_value_for_has_value_for.
+    eapply verilog_smt_match_states_partial_execution_defined_value_for.
+    apply verilog_smt_match_states_execution_of_valuation_same.
+    intros. apply Hhas_vars. apply Verilog.module_outputs_in_vars.
+    assumption.
+  - eapply verilog_smt_match_states_partial_execution_match_on.
+    setoid_rewrite <- Houtputs_permute.
+    eapply transfer_module_body_exec_valid.
+    + eassumption.
+    + rewrite Houtputs_permute. reflexivity.
+    + eassumption.
+    + eassumption.
+    + assert (H : SMT.execution_of_valuation tag m ρ // Verilog.module_inputs v =( Verilog.module_inputs v )= SMT.execution_of_valuation tag m ρ). {
+        apply RegisterState.match_on_limit_to_regs_iff.
+        apply RegisterState.limit_to_regs_twice.
+      }
+      rewrite H.
       apply verilog_smt_match_states_execution_of_valuation_same.
-      intros. apply Hhas_vars. apply Verilog.module_input_in_vars. assumption.
-    + apply defined_value_for_has_value_for.
-      eapply verilog_smt_match_states_partial_execution_defined_value_for.
-      apply verilog_smt_match_states_execution_of_valuation_same.
-      intros. apply Hhas_vars. apply Verilog.module_outputs_in_vars.
-      assumption.
-    + eapply verilog_smt_match_states_partial_execution_match_on.
-      setoid_rewrite <- Houtputs_permute. assumption.
+      auto using Verilog.module_input_in_vars.
 Qed.
 
 Lemma bij_gsi (m : VerilogSMTBijection.t) tag var smtName prf1 prf2 :
@@ -721,7 +647,7 @@ Proof.
   intros [e' [Hrun Hmatch]] Hin.
   unfold "_ =( _ )= _" in Hmatch.
   setoid_rewrite List.in_app_iff in Hmatch.
-  edestruct Hmatch as [xbv [He' He]]; eauto.
+  eauto.
 Qed.
 
 Lemma valid_execution_outputs_have_value v e var :
@@ -733,7 +659,7 @@ Proof.
   intros [e' [Hrun Hmatch]] Hin.
   unfold "_ =( _ )= _" in Hmatch.
   setoid_rewrite List.in_app_iff in Hmatch.
-  edestruct Hmatch as [xbv [He' He]]; eauto.
+  eauto.
 Qed.
 
 Lemma valid_execution_complete v : forall e,
@@ -792,96 +718,6 @@ Proof.
     + eapply transfer_module_body_satisfiable; eassumption.
 Qed.
 
-(* Lemma defined_value_for_impl C1 C2 e :
- *   (forall var, C2 var -> C1 var) ->
- *   RegisterState.defined_value_for C1 e ->
- *   RegisterState.defined_value_for C2 e.
- * Proof. unfold defined_value_for. firstorder. Qed. *)
-
-Definition defined_value_for_all := RegisterState.defined_value_for (fun _ => True).
-
-Lemma exec_module_item_no_exes C tag m t regs inputs outputs mi : forall regs',
-    transfer_module_item tag m inputs outputs mi = inr t ->
-    exec_module_item regs mi = Some regs' ->
-    RegisterState.defined_value_for (fun var => C var \/ List.In var (Verilog.module_item_reads mi)) regs ->
-    RegisterState.defined_value_for (fun var => C var \/ List.In var (Verilog.module_item_reads mi) \/ List.In var (Verilog.module_item_writes mi)) regs'.
-Proof.
-  funelim (transfer_module_item tag m inputs outputs mi).
-  all: clear Heqcall.
-  all: intros.
-  all: try discriminate; expect 1.
-  simp
-      transfer_module_item
-      exec_module_item
-      exec_statement
-      module_item_reads
-      statement_reads
-      expr_reads in *.
-  monad_inv.
-  simp module_item_writes statement_writes expr_reads. simpl.
-  unfold RegisterState.defined_value_for.
-  intros var' Hvar_in'.
-  destruct (dec (var' = var)).
-  - subst.
-    rewrite RegisterState.set_reg_get_in.
-    edestruct eval_expr_defined; expect 2. {
-      setoid_replace
-        (fun v : Verilog.variable => List.In v (Verilog.expr_reads rhs))
-	with
-        (fun v : Verilog.variable => C v \/ List.In v (Verilog.expr_reads rhs))
-	by crush.
-      eassumption.
-    }
-    rewrite <- E3. crush.
-  - assert (C var' \/ List.In var' (Verilog.expr_reads rhs)) by crush. clear Hvar_in'.
-    rewrite RegisterState.set_reg_get_out by congruence.
-    eauto.
-Qed.
-
-Lemma exec_module_body_no_exes body : forall C tag m inputs outputs t regs regs',
-  transfer_module_body tag m inputs outputs body = inr t ->
-  exec_module_body regs body = Some regs' ->
-  RegisterState.defined_value_for
-    (fun var => C var
-             \/ List.In var (Verilog.module_body_reads body))
-    regs ->
-  RegisterState.defined_value_for
-    (fun var => C var
-             \/ List.In var (Verilog.module_body_writes body)
-             \/ List.In var (Verilog.module_body_reads body))
-    regs'.
-Proof.
-  induction body;
-    simpl in *; intros * Htransfer Hrun Hdefined.
-  - simp exec_module_body transfer_module_body module_body_reads in *.
-    inv Hrun. intros var Hvar_in.
-    simp module_body_writes in *. crush.
-  -
-    simp
-      transfer_module_body
-      exec_module_body
-      module_body_reads
-    in *.
-    monad_inv.
-    simp module_body_writes.
-    setoid_rewrite List.in_app_iff.
-    rewrite <- ! RegisterState.defined_value_for_split_iff.
-    RegisterState.unpack_defined_value_for.
-    pose proof (exec_module_item_no_exes
-                  (fun v => C v
-                         \/ List.In v (Verilog.module_body_reads body)))
-      as Ha.
-    specialize (IHbody (fun var => C var
-                                \/ List.In var (Verilog.module_item_reads a)
-                                \/ List.In var (Verilog.module_item_writes a))).
-    simpl in *.
-    RegisterState.unpack_defined_value_for.
-    insterU Ha. RegisterState.unpack_defined_value_for.
-    insterU IHbody. simpl in IHbody.
-    RegisterState.unpack_defined_value_for.
-    repeat split; assumption.
-Qed.
-
 Lemma defined_value_for_execution_match_on C e' e :
   e' ={ C }= e ->
   RegisterState.defined_value_for C e' ->
@@ -902,33 +738,24 @@ Lemma valid_execution_no_exes_written v : forall e tag start q,
     RegisterState.defined_value_for (fun var => List.In var (Verilog.module_body_writes (Verilog.modBody v))) e.
 Proof.
   unfold valid_execution, all_vars_driven.
-  intros * Htransf [e' [Hrun [Hinput_has_value [Houtput_has_value Hmatch]]]] Hinputs_defined.
+  intros * Htransf [Hinput_has_value [Houtput_has_value Hmatch]] Hinputs_defined.
   unfold verilog_to_smt in Htransf. monad_inv.
-  assert
-    (RegisterState.defined_value_for
-       (fun var : Verilog.variable =>
-          List.In var (Verilog.module_inputs v)
-          \/ List.In var (Verilog.module_body_reads (Verilog.modBody v)))
-       (RegisterState.limit_to_regs (Verilog.module_inputs v) e)) as Hdefined_initial. {
-    unfold list_subset in *. rewrite List.Forall_forall in *.
-    unfold RegisterState.limit_to_regs, RegisterState.defined_value_for.
-    intros var [|]; autodestruct; crush.
-  }
-  rename_match (list_subset (Verilog.module_body_reads (Verilog.modBody v)) (Verilog.module_inputs v)) into Hreads_in_inputs.
-  rename_match (Permutation (Verilog.module_body_writes (Verilog.modBody v)) (Verilog.module_outputs v)) into Hwrites_outputs_permute.
-  unfold run_vmodule, mk_initial_state in Hrun.
-  rewrite sort_module_items_stable in Hrun by assumption. simpl in Hrun.
-  pose proof (exec_module_body_no_exes
-               (Verilog.modBody v)
-               (fun var => List.In var (Verilog.module_inputs v))) as H.
-  simpl in *.
-  rewrite RegisterState.limit_to_regs_twice in *.
-  insterU H.
+  rename_match (module_items_sorted _ _) into Hsorted.
+  rename_match (Permutation _ _) into Hout_permute.
+  unfold run_vmodule in Hmatch.
+  rewrite sort_module_items_stable in Hmatch by apply Hsorted.
   RegisterState.unpack_match_on.
-  RegisterState.unpack_defined_value_for.
-  rename_match (e' =( Verilog.module_outputs v )= e) into Hmatch_outputs.
-  setoid_rewrite Hwrites_outputs_permute.
-  setoid_rewrite <- Hmatch_outputs.
-  setoid_rewrite <- Hwrites_outputs_permute.
-  assumption.
+  rename_match (exec_module_body _ _ =( Verilog.module_outputs _ )= _) into Hmatch_out.
+  setoid_rewrite <- Hout_permute in Hmatch_out.
+  rewrite <- Hmatch_out.
+  apply Clean.exec_module_body_defined with (l_before := Verilog.module_inputs v).
+  - assumption.
+  - apply list_subset_app_r.
+  - unfold mk_initial_state.
+    rewrite RegisterState.limit_to_regs_twice in *.
+    assert (Hdrop_limit : e // Verilog.module_inputs v =( Verilog.module_inputs v )= e). {
+        apply RegisterState.match_on_limit_to_regs_iff.
+        apply RegisterState.limit_to_regs_twice.
+    } rewrite Hdrop_limit.
+    apply Hinputs_defined.
 Qed.
